src/Parsers/MinimalParseOfParse.v
@@ -3,6 +3,7 @@ Require Import Coq.Strings.String Coq.Lists.List Coq.Program.Program Coq.Classes
 Require Import Coq.omega.Omega.
 Require Import Coq.Program.Wf Coq.Arith.Wf_nat.
 Require Import ADTSynthesis.Parsers.ContextFreeGrammar ADTSynthesis.Parsers.ContextFreeGrammarProperties ADTSynthesis.Parsers.WellFoundedParse.
+Require Import ADTSynthesis.Parsers.BooleanBaseTypes ADTSynthesis.Parsers.BaseTypes.
 Require Export ADTSynthesis.Parsers.MinimalParse.
 Require Import ADTSynthesis.Common ADTSynthesis.Common.Wf.
 
@@ -12,37 +13,16 @@ Local Open Scope string_like_scope.
 Local Notation "f ∘ g" := (fun x => f (g x)).
 
 Section cfg.
-  Context CharType (String : string_like CharType) (G : grammar CharType).
-  Context (names_listT : Type)
-          (initial_names_data : names_listT)
-          (is_valid_name : names_listT -> string -> bool)
-          (remove_name : names_listT -> string -> names_listT)
-          (names_listT_R : names_listT -> names_listT -> Prop)
-          (remove_name_dec : forall ls name,
-                               is_valid_name ls name = true
-                               -> names_listT_R (remove_name ls name) ls)
-          (remove_name_1
-           : forall ls ps ps',
-               is_valid_name (remove_name ls ps) ps' = true
-               -> is_valid_name ls ps' = true)
-          (remove_name_2
-           : forall ls ps ps',
-               is_valid_name (remove_name ls ps) ps' = false
-               <-> is_valid_name ls ps' = false \/ ps = ps')
-          (ntl_wf : well_founded names_listT_R).
-
-  Context (names_listT_R_respectful : forall x y,
-                                        sub_names_listT is_valid_name x y
+  Context {CharType} {String : string_like CharType} {G : grammar CharType}.
+  Context `{predata : parser_computational_predataT}
+          `{rdata' : @parser_removal_dataT' predata}.
+  Context (nonterminals_listT_R_respectful : forall x y,
+                                        sub_nonterminals_listT x y
                                         -> x <> y
-                                        -> names_listT_R x y).
-
-  Local Notation minimal_parse_of_production := (@minimal_parse_of_production CharType String G names_listT initial_names_data is_valid_name remove_name).
-  Local Notation minimal_parse_of := (@minimal_parse_of CharType String G names_listT initial_names_data is_valid_name remove_name).
-  Local Notation minimal_parse_of_name := (@minimal_parse_of_name CharType String G names_listT initial_names_data is_valid_name remove_name).
-  Local Notation minimal_parse_of_item := (@minimal_parse_of_item CharType String G names_listT initial_names_data is_valid_name remove_name).
+                                        -> nonterminals_listT_R x y).
 
   Lemma strle_from_min_parse_of_production {str0 valid strs pats}
-        (p1 : minimal_parse_of_production str0 valid strs pats)
+        (p1 : minimal_parse_of_production (String := String) (G := G) str0 valid strs pats)
   : strs ≤s str0.
   Proof.
     destruct p1; trivial; [].
@@ -53,17 +33,17 @@ Section cfg.
     eauto using Empty_Length with arith.
   Qed.
 
-  Definition parse_of_item_name__of__minimal_parse_of_name'
+  Definition parse_of_item_nonterminal__of__minimal_parse_of_nonterminal'
              (parse_of__of__minimal_parse_of
               : forall str0 valid str prods,
-                  @minimal_parse_of str0 valid str prods -> parse_of String G str prods)
-             {str0 valid str name} (p : @minimal_parse_of_name str0 valid str name)
-  : parse_of_item String G str (NonTerminal _ name)
+                  minimal_parse_of (String := String) (G := G) str0 valid str prods -> parse_of String G str prods)
+             {str0 valid str nonterminal} (p : minimal_parse_of_nonterminal (String := String) (G := G) str0 valid str nonterminal)
+  : parse_of_item String G str (NonTerminal _ nonterminal)
     := ParseNonTerminal
-         name
+         nonterminal
          (@parse_of__of__minimal_parse_of
             _ _ _ _
-            (match p as p in (@MinimalParse.minimal_parse_of_name _ _ _ _ _ _ _ str0 valid str name)
+            (match p as p in (@MinimalParse.minimal_parse_of_nonterminal _ _ _ _ str0 valid str nonterminal)
                    return minimal_parse_of (match p with
                                               | MinParseNonTerminalStrLt _ _ _ _ _ _ _ => _
                                               | MinParseNonTerminalStrEq _ _ _ _ _ _ => _
@@ -72,25 +52,25 @@ Section cfg.
                                               | MinParseNonTerminalStrLt _ _ _ _ _ _ _ => _
                                               | MinParseNonTerminalStrEq _ _ _ _ _ _ => _
                                             end)
-                                           str (Lookup G name) with
-               | MinParseNonTerminalStrLt str0 valid name str pf pf' p' => p'
-               | MinParseNonTerminalStrEq str valid name H H' p' => p'
+                                           str (Lookup G nonterminal) with
+               | MinParseNonTerminalStrLt str0 valid nonterminal str pf pf' p' => p'
+               | MinParseNonTerminalStrEq str valid nonterminal H H' p' => p'
              end)).
 
   Definition parse_of_item__of__minimal_parse_of_item'
              (parse_of__of__minimal_parse_of
               : forall str0 valid str prods,
-                  @minimal_parse_of str0 valid str prods -> parse_of String G str prods)
-             {str0 valid str it} (p : @minimal_parse_of_item str0 valid str it)
+                  minimal_parse_of (String := String) (G := G) str0 valid str prods -> parse_of String G str prods)
+             {str0 valid str it} (p : minimal_parse_of_item (String := String) (G := G) str0 valid str it)
   : parse_of_item String G str it
-    := match p in (@MinimalParse.minimal_parse_of_item _ _ _ _ _ _ _ str0 valid str it) return parse_of_item String G str it with
+    := match p in (MinimalParse.minimal_parse_of_item str0 valid str it) return parse_of_item String G str it with
          | MinParseTerminal str0 valid x
            => ParseTerminal String G x
          | MinParseNonTerminal str0 valid _ _ p'
-           => @parse_of_item_name__of__minimal_parse_of_name' (@parse_of__of__minimal_parse_of) _ _ _ _ p'
+           => @parse_of_item_nonterminal__of__minimal_parse_of_nonterminal' (@parse_of__of__minimal_parse_of) _ _ _ _ p'
        end.
 
-  Fixpoint parse_of__of__minimal_parse_of {str0 valid str pats} (p : @minimal_parse_of str0 valid str pats)
+  Fixpoint parse_of__of__minimal_parse_of {str0 valid str pats} (p : minimal_parse_of (String := String) (G := G) str0 valid str pats)
   : parse_of String G str pats
     := match p with
          | MinParseHead str0 valid str pat pats p'
@@ -98,7 +78,7 @@ Section cfg.
          | MinParseTail str0 valid str pat pats p'
            => ParseTail pat (parse_of__of__minimal_parse_of p')
        end
-  with parse_of_production__of__minimal_parse_of_production {str0 valid str pat} (p : @minimal_parse_of_production str0 valid str pat)
+  with parse_of_production__of__minimal_parse_of_production {str0 valid str pat} (p : minimal_parse_of_production (String := String) (G := G) str0 valid str pat)
        : parse_of_production String G str pat
        := match p with
             | MinParseProductionNil str0 valid
@@ -109,25 +89,25 @@ Section cfg.
                    (parse_of_production__of__minimal_parse_of_production p'')
           end.
 
-  Definition parse_of_item_name__of__minimal_parse_of_name
-  : forall {str0 valid str name} (p : @minimal_parse_of_name str0 valid str name),
-      parse_of_item String G str (NonTerminal _ name)
-    := @parse_of_item_name__of__minimal_parse_of_name' (@parse_of__of__minimal_parse_of).
+  Definition parse_of_item_nonterminal__of__minimal_parse_of_nonterminal
+  : forall {str0 valid str nonterminal} (p : minimal_parse_of_nonterminal (String := String) (G := G) str0 valid str nonterminal),
+      parse_of_item String G str (NonTerminal _ nonterminal)
+    := @parse_of_item_nonterminal__of__minimal_parse_of_nonterminal' (@parse_of__of__minimal_parse_of).
 
   Definition parse_of_item__of__minimal_parse_of_item
   : forall {str0 valid str it},
-      @minimal_parse_of_item str0 valid str it
+      minimal_parse_of_item (String := String) (G := G) str0 valid str it
       -> parse_of_item String G str it
     := @parse_of_item__of__minimal_parse_of_item' (@parse_of__of__minimal_parse_of).
 
   Section contract.
-    Local Hint Constructors MinimalParse.minimal_parse_of_name.
+    Local Hint Constructors MinimalParse.minimal_parse_of_nonterminal.
 
-    Definition contract_minimal_parse_of_name_lt
-               {str0 str valid valid' name}
+    Definition contract_minimal_parse_of_nonterminal_lt
+               {str0 str valid valid' nonterminal}
                (Hlt : Length str < Length str0)
-               (p : @minimal_parse_of_name str0 valid str name)
-    : @minimal_parse_of_name str0 valid' str name.
+               (p : minimal_parse_of_nonterminal (String := String) (G := G) str0 valid str nonterminal)
+    : minimal_parse_of_nonterminal (String := String) (G := G) str0 valid' str nonterminal.
     Proof.
       destruct p.
       { constructor (assumption). }
@@ -137,19 +117,19 @@ Section cfg.
     Definition contract_minimal_parse_of_item_lt
                {str0 str valid valid' it}
                (Hlt : Length str < Length str0)
-               (p : @minimal_parse_of_item str0 valid str it)
-    : @minimal_parse_of_item str0 valid' str it.
+               (p : minimal_parse_of_item (String := String) (G := G) str0 valid str it)
+    : minimal_parse_of_item (String := String) (G := G) str0 valid' str it.
     Proof.
       destruct p as [p|p].
       { constructor. }
-      { constructor (eapply contract_minimal_parse_of_name_lt; eassumption). }
+      { constructor (eapply contract_minimal_parse_of_nonterminal_lt; eassumption). }
     Defined.
 
     Definition contract_minimal_parse_of_production_lt
                {str0 str valid valid' pat}
                (Hlt : Length str < Length str0)
-               (p : @minimal_parse_of_production str0 valid str pat)
-    : @minimal_parse_of_production str0 valid' str pat.
+               (p : minimal_parse_of_production (String := String) (G := G) str0 valid str pat)
+    : minimal_parse_of_production (String := String) (G := G) str0 valid' str pat.
     Proof.
       induction p.
       { constructor. }
@@ -167,8 +147,8 @@ Section cfg.
     Definition contract_minimal_parse_of_lt
                {str0 str valid valid' pats}
                (Hlt : Length str < Length str0)
-               (p : @minimal_parse_of str0 valid str pats)
-    : @minimal_parse_of str0 valid' str pats.
+               (p : minimal_parse_of (String := String) (G := G) str0 valid str pats)
+    : minimal_parse_of (String := String) (G := G) str0 valid' str pats.
     Proof.
       induction p.
       { constructor (eapply contract_minimal_parse_of_production_lt; eassumption). }
@@ -177,16 +157,16 @@ Section cfg.
 
     Section contract_eq.
       Lemma parse_of_contract_minimal_parse_of_item_lt
-            {str0 str : String} {valid valid' : names_listT}
+            {str0 str : String} {valid valid' : nonterminals_listT}
             {Hlt : Length str < Length str0}
             {it}
-            (p : @minimal_parse_of_item str0 valid str it)
+            (p : minimal_parse_of_item (String := String) (G := G) str0 valid str it)
       : parse_of_item__of__minimal_parse_of_item
           (contract_minimal_parse_of_item_lt (valid' := valid') Hlt p)
         = parse_of_item__of__minimal_parse_of_item p.
       Proof.
-        destruct_head MinimalParse.minimal_parse_of_item; simpl; try reflexivity.
-        destruct_head MinimalParse.minimal_parse_of_name; try reflexivity.
+        destruct_head @MinimalParse.minimal_parse_of_item; simpl; try reflexivity.
+        destruct_head @MinimalParse.minimal_parse_of_nonterminal; try reflexivity.
         unfold False_rect.
         match goal with
           | [ |- appcontext[match ?e with end] ] => destruct e
@@ -194,10 +174,10 @@ Section cfg.
       Qed.
 
       Lemma parse_of_contract_minimal_parse_of_production_lt
-            {str0 str : String} {valid valid' : names_listT}
+            {str0 str : String} {valid valid' : nonterminals_listT}
             {Hlt : Length str < Length str0}
             {pat}
-            (p : @minimal_parse_of_production str0 valid str pat)
+            (p : minimal_parse_of_production (String := String) (G := G) str0 valid str pat)
       : parse_of_production__of__minimal_parse_of_production
           (contract_minimal_parse_of_production_lt (valid' := valid') Hlt p)
         = parse_of_production__of__minimal_parse_of_production p.
@@ -208,10 +188,10 @@ Section cfg.
       Qed.
 
       Lemma parse_of_contract_minimal_parse_of_lt
-            {str0 str : String} {valid valid' : names_listT}
+            {str0 str : String} {valid valid' : nonterminals_listT}
             {Hlt : Length str < Length str0}
             {pats}
-            (p : @minimal_parse_of str0 valid str pats)
+            (p : minimal_parse_of (String := String) (G := G) str0 valid str pats)
       : parse_of__of__minimal_parse_of
           (contract_minimal_parse_of_lt (valid' := valid') Hlt p)
         = parse_of__of__minimal_parse_of p.
@@ -224,27 +204,27 @@ Section cfg.
   End contract.
 
   (** Re-add this so rewrite works *)
-  Global Add Parametric Morphism : remove_name
-  with signature (sub_names_listT is_valid_name) ==> eq ==> (sub_names_listT is_valid_name)
-    as remove_name_mor.
+  Global Add Parametric Morphism : remove_nonterminal
+  with signature sub_nonterminals_listT ==> eq ==> sub_nonterminals_listT
+    as remove_nonterminal_mor.
   Proof.
-    intros; apply (@remove_name_mor); try assumption; reflexivity.
+    intros; apply (@remove_nonterminal_mor); try assumption; reflexivity.
   Qed.
 
-  Definition expand_minimal_parse_of_name'
+  Definition expand_minimal_parse_of_nonterminal'
              (expand_minimal_parse_of
               : forall {str0 str0' valid valid' str prods}
                        (Hstr : str0 ≤s str0')
-                       (H : sub_names_listT is_valid_name valid valid')
-                       (Hinit : sub_names_listT is_valid_name valid' initial_names_data)
-                       (p : @minimal_parse_of str0 valid str prods),
-                  @minimal_parse_of str0' valid' str prods)
-             {str0 str0' valid valid' str name}
+                       (H : sub_nonterminals_listT valid valid')
+                       (Hinit : sub_nonterminals_listT valid' initial_nonterminals_data)
+                       (p : minimal_parse_of (String := String) (G := G) str0 valid str prods),
+                  minimal_parse_of (String := String) (G := G) str0' valid' str prods)
+             {str0 str0' valid valid' str nonterminal}
              (Hstr : str0 ≤s str0')
-             (H : sub_names_listT is_valid_name valid valid')
-             (Hinit : sub_names_listT is_valid_name valid' initial_names_data)
-             (p : @minimal_parse_of_name str0 valid str name)
-  : @minimal_parse_of_name str0' valid' str name.
+             (H : sub_nonterminals_listT valid valid')
+             (Hinit : sub_nonterminals_listT valid' initial_nonterminals_data)
+             (p : minimal_parse_of_nonterminal (String := String) (G := G) str0 valid str nonterminal)
+  : minimal_parse_of_nonterminal (String := String) (G := G) str0' valid' str nonterminal.
   Proof.
     destruct p;
     first [ apply MinParseNonTerminalStrLt;
@@ -259,7 +239,7 @@ Section cfg.
             | eapply expand_minimal_parse_of; [ .. | eassumption ];
               solve [ reflexivity
                     | rewrite ?H, ?Hinit;
-                      eauto using sub_names_listT_remove;
+                      eauto using sub_nonterminals_listT_remove;
                       reflexivity ] ]. }
   Defined.
 
@@ -267,35 +247,35 @@ Section cfg.
              (expand_minimal_parse_of
               : forall {str0 str0' valid valid' str prods}
                        (Hstr : str0 ≤s str0')
-                       (H : sub_names_listT is_valid_name valid valid')
-                       (Hinit : sub_names_listT is_valid_name valid' initial_names_data)
-                       (p : @minimal_parse_of str0 valid str prods),
-                  @minimal_parse_of str0' valid' str prods)
+                       (H : sub_nonterminals_listT valid valid')
+                       (Hinit : sub_nonterminals_listT valid' initial_nonterminals_data)
+                       (p : minimal_parse_of (String := String) (G := G) str0 valid str prods),
+                  minimal_parse_of (String := String) (G := G) str0' valid' str prods)
              {str0 str0' valid valid' str it}
              (Hstr : str0 ≤s str0')
-             (H : sub_names_listT is_valid_name valid valid')
-             (Hinit : sub_names_listT is_valid_name valid' initial_names_data)
-             (p : @minimal_parse_of_item str0 valid str it)
-  : @minimal_parse_of_item str0' valid' str it.
+             (H : sub_nonterminals_listT valid valid')
+             (Hinit : sub_nonterminals_listT valid' initial_nonterminals_data)
+             (p : minimal_parse_of_item (String := String) (G := G) str0 valid str it)
+  : minimal_parse_of_item (String := String) (G := G) str0' valid' str it.
   Proof.
     destruct p.
     { apply MinParseTerminal. }
     { apply MinParseNonTerminal; [].
-      eapply expand_minimal_parse_of_name'; [..| eassumption ];
+      eapply expand_minimal_parse_of_nonterminal'; [..| eassumption ];
       try assumption. }
   Defined.
 
   Fixpoint expand_minimal_parse_of
            {str0 str0' valid valid' str pats}
            (Hstr : str0 ≤s str0')
-           (H : sub_names_listT is_valid_name valid valid')
-           (Hinit : sub_names_listT is_valid_name valid' initial_names_data)
-           (p : @minimal_parse_of str0 valid str pats)
-  : @minimal_parse_of str0' valid' str pats
-    := match p in (@MinimalParse.minimal_parse_of _ _ _ _ _ _ _ str0 valid str pats)
+           (H : sub_nonterminals_listT valid valid')
+           (Hinit : sub_nonterminals_listT valid' initial_nonterminals_data)
+           (p : minimal_parse_of (String := String) (G := G) str0 valid str pats)
+  : minimal_parse_of (String := String) (G := G) str0' valid' str pats
+    := match p in (MinimalParse.minimal_parse_of str0 valid str pats)
              return (str0 ≤s str0'
-                     -> sub_names_listT is_valid_name valid valid'
-                     -> @minimal_parse_of str0' valid' str pats)
+                     -> sub_nonterminals_listT valid valid'
+                     -> minimal_parse_of (String := String) (G := G) str0' valid' str pats)
        with
          | MinParseHead str0 valid str pat pats p'
            => fun Hstr H => MinParseHead pats (expand_minimal_parse_of_production Hstr H Hinit p')
@@ -305,15 +285,15 @@ Section cfg.
   with expand_minimal_parse_of_production
          {str0 str0' valid valid' str pat}
          (Hstr : str0 ≤s str0')
-         (H : sub_names_listT is_valid_name valid valid')
-         (Hinit : sub_names_listT is_valid_name valid' initial_names_data)
-         (p : @minimal_parse_of_production str0 valid str pat)
-       : @minimal_parse_of_production str0' valid' str pat
-       := match p in (@MinimalParse.minimal_parse_of_production _ _ _ _ _ _ _ str0 valid str pats)
-                return (str0 ≤s str0' -> sub_names_listT is_valid_name valid valid' -> minimal_parse_of_production str0' valid' str pats)
+         (H : sub_nonterminals_listT valid valid')
+         (Hinit : sub_nonterminals_listT valid' initial_nonterminals_data)
+         (p : minimal_parse_of_production (String := String) (G := G) str0 valid str pat)
+       : minimal_parse_of_production (String := String) (G := G) str0' valid' str pat
+       := match p in (MinimalParse.minimal_parse_of_production str0 valid str pats)
+                return (str0 ≤s str0' -> sub_nonterminals_listT valid valid' -> minimal_parse_of_production str0' valid' str pats)
           with
             | MinParseProductionNil str0 valid
-              => fun _ _ => MinimalParse.MinParseProductionNil _ _ _ _ _ _ _
+              => fun _ _ => MinimalParse.MinParseProductionNil _ _
             | MinParseProductionCons str0 valid str strs pat pats pf p' p''
               => fun Hstr H => MinParseProductionCons
                                  (transitivity pf Hstr)
@@ -321,35 +301,35 @@ Section cfg.
                                  (expand_minimal_parse_of_production Hstr H Hinit p'')
           end Hstr H.
 
-  Definition expand_minimal_parse_of_name
-  : forall {str0 str0' valid valid' str name}
+  Definition expand_minimal_parse_of_nonterminal
+  : forall {str0 str0' valid valid' str nonterminal}
            (Hstr : str0 ≤s str0')
-           (H : sub_names_listT is_valid_name valid valid')
-           (Hinit : sub_names_listT is_valid_name valid' initial_names_data)
-           (p : @minimal_parse_of_name str0 valid str name),
-      @minimal_parse_of_name str0' valid' str name
-    := @expand_minimal_parse_of_name' (@expand_minimal_parse_of).
+           (H : sub_nonterminals_listT valid valid')
+           (Hinit : sub_nonterminals_listT valid' initial_nonterminals_data)
+           (p : minimal_parse_of_nonterminal (String := String) (G := G) str0 valid str nonterminal),
+      minimal_parse_of_nonterminal (String := String) (G := G) str0' valid' str nonterminal
+    := @expand_minimal_parse_of_nonterminal' (@expand_minimal_parse_of).
 
   Definition expand_minimal_parse_of_item
   : forall {str0 str0' valid valid' str it}
            (Hstr : str0 ≤s str0')
-           (H : sub_names_listT is_valid_name valid valid')
-           (Hinit : sub_names_listT is_valid_name valid' initial_names_data)
-           (p : @minimal_parse_of_item str0 valid str it),
-      @minimal_parse_of_item str0' valid' str it
+           (H : sub_nonterminals_listT valid valid')
+           (Hinit : sub_nonterminals_listT valid' initial_nonterminals_data)
+           (p : minimal_parse_of_item (String := String) (G := G) str0 valid str it),
+      minimal_parse_of_item (String := String) (G := G) str0' valid' str it
     := @expand_minimal_parse_of_item' (@expand_minimal_parse_of).
 
   Section minimize.
     Let P : String -> string -> Prop
-      := fun _ p => is_valid_name initial_names_data p = true.
+      := fun _ p => is_valid_nonterminal initial_nonterminals_data p = true.
 
     Let alt_option h valid str
-      := { name : _ & (is_valid_name valid name = false /\ P str name)
-                      * { p : parse_of String G str (Lookup G name)
+      := { nonterminal : _ & (is_valid_nonterminal valid nonterminal = false /\ P str nonterminal)
+                      * { p : parse_of String G str (Lookup G nonterminal)
                               & (size_of_parse p < h)
                                 * Forall_parse_of P p } }%type.
 
-    Lemma not_alt_all {h str} (ps : alt_option h initial_names_data str)
+    Lemma not_alt_all {h str} (ps : alt_option h initial_nonterminals_data str)
     : False.
     Proof.
       subst P; simpl in *.
@@ -358,7 +338,7 @@ Section cfg.
       congruence.
     Qed.
 
-    Definition alt_all_elim {h str T} (ps : T + alt_option h initial_names_data str)
+    Definition alt_all_elim {h str T} (ps : T + alt_option h initial_nonterminals_data str)
     : T.
     Proof.
       destruct ps as [|ps]; [ assumption | exfalso ].
@@ -366,7 +346,7 @@ Section cfg.
     Defined.
 
     Definition expand_alt_option' {h h' str str' valid valid'}
-               (H : h <= h') (H' : sub_names_listT is_valid_name valid' valid) (H'' : str = str')
+               (H : h <= h') (H' : sub_nonterminals_listT valid' valid) (H'' : str = str')
     : alt_option h valid str -> alt_option h' valid' str'.
     Proof.
       hnf in H'; unfold alt_option.
@@ -393,7 +373,7 @@ Section cfg.
     Defined.
 
     Definition expand_alt_option {h h' str str' valid valid'}
-               (H : h < h') (H' : sub_names_listT is_valid_name valid' valid) (H'' : str = str')
+               (H : h < h') (H' : sub_nonterminals_listT valid' valid) (H'' : str = str')
     : alt_option h valid str -> alt_option h' valid' str'.
     Proof.
       apply expand_alt_option'; try assumption.
@@ -403,12 +383,12 @@ Section cfg.
     Section wf_parts.
       Let of_parse_item_T' h
           {str0 str : String} (pf : str ≤s str0)
-          (valid : names_listT) {it : item CharType}
+          (valid : nonterminals_listT) {it : item CharType}
           (p : parse_of_item String G str it)
         := forall (p_small : size_of_parse_item p < h),
-             sub_names_listT is_valid_name valid initial_names_data
+             sub_nonterminals_listT valid initial_nonterminals_data
              -> Forall_parse_of_item P p
-             -> ({ p' : @minimal_parse_of_item str0 valid str it
+             -> ({ p' : minimal_parse_of_item (String := String) (G := G) str0 valid str it
                         & (size_of_parse_item (parse_of_item__of__minimal_parse_of_item p') <= size_of_parse_item p)
                           * Forall_parse_of_item P (parse_of_item__of__minimal_parse_of_item p') })%type
                 + alt_option (size_of_parse_item p) valid str.
@@ -418,12 +398,12 @@ Section cfg.
 
       Let of_parse_production_T' h
           {str0 str : String} (pf : str ≤s str0)
-          (valid : names_listT) {pat : production CharType}
+          (valid : nonterminals_listT) {pat : production CharType}
           (p : parse_of_production String G str pat)
         := forall (p_small : size_of_parse_production p < h),
-             sub_names_listT is_valid_name valid initial_names_data
+             sub_nonterminals_listT valid initial_nonterminals_data
              -> Forall_parse_of_production P p
-             -> ({ p' : @minimal_parse_of_production str0 valid str pat
+             -> ({ p' : minimal_parse_of_production (String := String) (G := G) str0 valid str pat
                         & (size_of_parse_production (parse_of_production__of__minimal_parse_of_production p') <= size_of_parse_production p)
                           * Forall_parse_of_production P (parse_of_production__of__minimal_parse_of_production p') })%type
                 + alt_option (size_of_parse_production p) valid str.
@@ -433,12 +413,12 @@ Section cfg.
 
       Let of_parse_T' h
           {str0 str : String} (pf : str ≤s str0)
-          (valid : names_listT) {pats : productions CharType}
+          (valid : nonterminals_listT) {pats : productions CharType}
           (p : parse_of String G str pats)
         := forall (p_small : size_of_parse p < h),
-             sub_names_listT is_valid_name valid initial_names_data
+             sub_nonterminals_listT valid initial_nonterminals_data
              -> Forall_parse_of P p
-             -> ({ p' : @minimal_parse_of str0 valid str pats
+             -> ({ p' : minimal_parse_of (String := String) (G := G) str0 valid str pats
                         & (size_of_parse (parse_of__of__minimal_parse_of p') <= size_of_parse p)
                           * Forall_parse_of P (parse_of__of__minimal_parse_of p') })%type
                 + alt_option (size_of_parse p) valid str.
@@ -446,34 +426,34 @@ Section cfg.
       Let of_parse_T str0 h
         := forall str pf valid pats p, @of_parse_T' h str0 str pf valid pats p.
 
-      Let of_parse_name_T {str0 str valid name} (p : parse_of String G str (Lookup G name)) h
-        := size_of_parse_item (ParseNonTerminal name p) < h
+      Let of_parse_nonterminal_T {str0 str valid nonterminal} (p : parse_of String G str (Lookup G nonterminal)) h
+        := size_of_parse_item (ParseNonTerminal nonterminal p) < h
            -> str ≤s str0
-           -> sub_names_listT is_valid_name valid initial_names_data
-           -> Forall_parse_of_item P (ParseNonTerminal name p)
-           -> ({ p' : @minimal_parse_of_name str0 valid str name
-                      & (size_of_parse_item (parse_of_item__of__minimal_parse_of_item (MinParseNonTerminal p')) <= size_of_parse_item (ParseNonTerminal name p))
+           -> sub_nonterminals_listT valid initial_nonterminals_data
+           -> Forall_parse_of_item P (ParseNonTerminal nonterminal p)
+           -> ({ p' : minimal_parse_of_nonterminal (String := String) (G := G) str0 valid str nonterminal
+                      & (size_of_parse_item (parse_of_item__of__minimal_parse_of_item (MinParseNonTerminal p')) <= size_of_parse_item (ParseNonTerminal nonterminal p))
                         * Forall_parse_of_item P (parse_of_item__of__minimal_parse_of_item (MinParseNonTerminal p')) })%type
-              + alt_option (size_of_parse_item (ParseNonTerminal name p)) valid str.
+              + alt_option (size_of_parse_item (ParseNonTerminal nonterminal p)) valid str.
 
       Section item.
-        Context {str0 str : String} {valid : names_listT}.
+        Context {str0 str : String} {valid : nonterminals_listT}.
 
         Definition minimal_parse_of_item__of__parse_of_item
                    h
-                   (minimal_parse_of_name__of__parse_of_name
-                    : forall h' (pf : h' < S (S h)) {str0 str valid name}
-                             (p : parse_of String G str (Lookup G name)),
-                        @of_parse_name_T str0 str valid name p h')
+                   (minimal_parse_of_nonterminal__of__parse_of_nonterminal
+                    : forall h' (pf : h' < S (S h)) {str0 str valid nonterminal}
+                             (p : parse_of String G str (Lookup G nonterminal)),
+                        @of_parse_nonterminal_T str0 str valid nonterminal p h')
         : of_parse_item_T str h.
         Proof.
           intros str' pf valid' pats p H_h Hinit' H_forall.
           destruct h as [|h']; [ exfalso; omega | ].
-          destruct p as [|name' str'' p'].
+          destruct p as [|nonterminal' str'' p'].
           { left.
-            eexists (@MinimalParse.MinParseTerminal _ _ _ _ _ _ _ _ _ _);
+            eexists (MinimalParse.MinParseTerminal _ _ _);
               split; simpl; constructor. }
-          { edestruct (fun pf => @minimal_parse_of_name__of__parse_of_name (S h') pf str _ valid' _ p') as [ [p'' H''] | p'' ];
+          { edestruct (fun pf => @minimal_parse_of_nonterminal__of__parse_of_nonterminal (S h') pf str _ valid' _ p') as [ [p'' H''] | p'' ];
             try solve [ repeat (apply Lt.lt_n_Sn || apply Lt.lt_S)
                       | exact Hinit'
                       | exact H_h
@@ -489,7 +469,7 @@ Section cfg.
       End item.
 
       Section production.
-        Context {str0 str : String} {valid : names_listT}.
+        Context {str0 str : String} {valid : nonterminals_listT}.
 
         Local Ltac min_parse_prod_t' :=
           idtac;
@@ -505,7 +485,7 @@ Section cfg.
             | [ |- context G[size_of_parse_production (ParseProductionCons ?a ?b)] ]
               => let G' := context G[S (size_of_parse_item a + size_of_parse_production b)] in
                  change G'
-            | [ H : alt_option _ initial_names_data _ |- _ ]
+            | [ H : alt_option _ initial_nonterminals_data _ |- _ ]
               => apply not_alt_all in H
             | [ p0 : minimal_parse_of_item _ _ ?s0 ?pat,
                      p1 : minimal_parse_of_production _ _ ?s1 ?pats,
@@ -597,10 +577,10 @@ Section cfg.
 
         Fixpoint minimal_parse_of_production__of__parse_of_production
                  h
-                 (minimal_parse_of_name__of__parse_of_name
-                  : forall h' (pf : h' < S (S h)) {str0 str valid name}
-                           (p : parse_of String G str (Lookup G name)),
-                      @of_parse_name_T str0 str valid name p h')
+                 (minimal_parse_of_nonterminal__of__parse_of_nonterminal
+                  : forall h' (pf : h' < S (S h)) {str0 str valid nonterminal}
+                           (p : parse_of String G str (Lookup G nonterminal)),
+                      @of_parse_nonterminal_T str0 str valid nonterminal p h')
                  {struct h}
         : of_parse_production_T str h.
         Proof.
@@ -609,10 +589,10 @@ Section cfg.
           destruct p as [| str' strs' str'' pat' p0' p1' ].
           { clear minimal_parse_of_production__of__parse_of_production.
             left.
-            eexists (@MinimalParse.MinParseProductionNil _ _ _ _ _ _ _ _ _);
+            eexists (@MinimalParse.MinParseProductionNil _ _ _ _ _ _);
               repeat (reflexivity || esplit). }
           { specialize (fun h' pf
-                        => @minimal_parse_of_name__of__parse_of_name
+                        => @minimal_parse_of_nonterminal__of__parse_of_nonterminal
                              h' (transitivity pf (Lt.lt_n_Sn _))).
             change (S ((size_of_parse_item p0')
                        + (size_of_parse_production p1'))
@@ -621,8 +601,8 @@ Section cfg.
             pose proof (Lt.le_lt_trans _ _ _ (Plus.le_plus_l _ _) H_h) as H_h0.
             pose proof (Lt.le_lt_trans _ _ _ (Plus.le_plus_r _ _) H_h) as H_h1.
             clear H_h.
-            pose proof (fun valid Hinit => @minimal_parse_of_item__of__parse_of_item _ h'  minimal_parse_of_name__of__parse_of_name _ (transitivity (str_le1_append _ _) pf) valid _ p0' H_h0 Hinit (fst H_forall)) as p_it.
-            pose proof (fun valid Hinit => @minimal_parse_of_production__of__parse_of_production h' minimal_parse_of_name__of__parse_of_name _ (transitivity (str_le2_append _ _) pf) valid _ p1' H_h1 Hinit (snd H_forall)) as p_prod.
+            pose proof (fun valid Hinit => @minimal_parse_of_item__of__parse_of_item _ h'  minimal_parse_of_nonterminal__of__parse_of_nonterminal _ (transitivity (str_le1_append _ _) pf) valid _ p0' H_h0 Hinit (fst H_forall)) as p_it.
+            pose proof (fun valid Hinit => @minimal_parse_of_production__of__parse_of_production h' minimal_parse_of_nonterminal__of__parse_of_nonterminal _ (transitivity (str_le2_append _ _) pf) valid _ p1' H_h1 Hinit (snd H_forall)) as p_prod.
             destruct (stringlike_dec str' (Empty _)), (stringlike_dec str'' (Empty _));
               subst.
             { (* empty, empty *)
@@ -631,21 +611,21 @@ Section cfg.
                 [ | | | ];
                 min_parse_prod_t. }
             { (* empty, nonempty *)
-              specialize (p_it initial_names_data (reflexivity _)); specialize (p_prod valid' Hinit').
+              specialize (p_it initial_nonterminals_data (reflexivity _)); specialize (p_prod valid' Hinit').
               destruct p_it as [ [ p0'' H0''] |], p_prod as [ [ p1'' H1'' ] |];
                 [ | | | ];
                 min_parse_prod_t;
                 min_parse_prod_pose_t;
                 min_parse_prod_t. }
             { (* nonempty, empty *)
-              specialize (p_it valid' Hinit'); specialize (p_prod initial_names_data (reflexivity _)).
+              specialize (p_it valid' Hinit'); specialize (p_prod initial_nonterminals_data (reflexivity _)).
               destruct p_it as [ [ p0'' H0''] |], p_prod as [ [ p1'' H1'' ] |];
                 [ | | | ];
                 min_parse_prod_t;
                 min_parse_prod_pose_t;
                 min_parse_prod_t. }
             { (* nonempty, nonempty *)
-              specialize (p_it initial_names_data (reflexivity _)); specialize (p_prod initial_names_data (reflexivity _)).
+              specialize (p_it initial_nonterminals_data (reflexivity _)); specialize (p_prod initial_nonterminals_data (reflexivity _)).
               destruct p_it as [ [ p0'' H0''] |], p_prod as [ [ p1'' H1'' ] |];
                 [ | | | ];
                 min_parse_prod_t;
@@ -655,14 +635,14 @@ Section cfg.
       End production.
 
       Section productions.
-        Context {str0 str : String} {valid : names_listT}.
+        Context {str0 str : String} {valid : nonterminals_listT}.
 
         Fixpoint minimal_parse_of_productions__of__parse_of_productions
                  h
-                 (minimal_parse_of_name__of__parse_of_name
-                  : forall h' (pf : h' < S h) {str0 str valid name}
-                           (p : parse_of String G str (Lookup G name)),
-                      @of_parse_name_T str0 str valid name p h')
+                 (minimal_parse_of_nonterminal__of__parse_of_nonterminal
+                  : forall h' (pf : h' < S h) {str0 str valid nonterminal}
+                           (p : parse_of String G str (Lookup G nonterminal)),
+                      @of_parse_nonterminal_T str0 str valid nonterminal p h')
                  {struct h}
         : of_parse_T str h.
         Proof.
@@ -670,7 +650,7 @@ Section cfg.
           destruct h as [|h']; [ exfalso; omega | ].
           destruct p as [str' pat pats p' | str' pat pats p'].
           { clear minimal_parse_of_productions__of__parse_of_productions.
-            edestruct (@minimal_parse_of_production__of__parse_of_production _ h' minimal_parse_of_name__of__parse_of_name _ pf valid' _ p') as [ [p'' p''H] | [name' H'] ];
+            edestruct (@minimal_parse_of_production__of__parse_of_production _ h' minimal_parse_of_nonterminal__of__parse_of_nonterminal _ pf valid' _ p') as [ [p'' p''H] | [nonterminal' H'] ];
             try solve [ exact (Lt.lt_S_n _ _ H_h)
                       | exact H_forall
                       | exact Hinit' ];
@@ -682,7 +662,7 @@ Section cfg.
                 solve [ exact (Le.le_n_S _ _ (fst p''H))
                       | exact (snd p''H) ]. }
             { right.
-              exists name'.
+              exists nonterminal'.
               split;
                 try solve [ exact (fst H') ];
                 [].
@@ -691,9 +671,9 @@ Section cfg.
                 try solve [ exact (snd (projT2 (snd H')))
                           | exact (Lt.lt_S _ _ (fst (projT2 (snd H')))) ]. } }
           { specialize (fun h' pf
-                        => @minimal_parse_of_name__of__parse_of_name
+                        => @minimal_parse_of_nonterminal__of__parse_of_nonterminal
                              h' (transitivity pf (Lt.lt_n_Sn _))).
-            edestruct (minimal_parse_of_productions__of__parse_of_productions h'  minimal_parse_of_name__of__parse_of_name _ pf valid' _ p') as [ [p'' p''H] | [name' H'] ];
+            edestruct (minimal_parse_of_productions__of__parse_of_productions h'  minimal_parse_of_nonterminal__of__parse_of_nonterminal _ pf valid' _ p') as [ [p'' p''H] | [nonterminal' H'] ];
             try solve [ exact (Lt.lt_S_n _ _ H_h)
                       | exact Hinit'
                       | exact H_forall ];
@@ -705,7 +685,7 @@ Section cfg.
                 solve [ exact (Le.le_n_S _ _ (fst p''H))
                       | exact (snd p''H) ]. }
             { right.
-              exists name'.
+              exists nonterminal'.
               split;
                 try solve [ exact (fst H') ];
                 [].
@@ -716,24 +696,24 @@ Section cfg.
         Defined.
       End productions.
 
-      Section name.
+      Section nonterminal.
         Section step.
-          Definition minimal_parse_of_name__of__parse_of_name_step
+          Definition minimal_parse_of_nonterminal__of__parse_of_nonterminal_step
                      h
-                     (minimal_parse_of_name__of__parse_of_name
-                      : forall h' (pf : h' < h) {str0 str valid name}
-                               (p : parse_of String G str (Lookup G name)),
-                          @of_parse_name_T str0 str valid name p h')
-                     {str0 str valid name}
-                     (p : parse_of String G str (Lookup G name))
-          : @of_parse_name_T str0 str valid name p h.
+                     (minimal_parse_of_nonterminal__of__parse_of_nonterminal
+                      : forall h' (pf : h' < h) {str0 str valid nonterminal}
+                               (p : parse_of String G str (Lookup G nonterminal)),
+                          @of_parse_nonterminal_T str0 str valid nonterminal p h')
+                     {str0 str valid nonterminal}
+                     (p : parse_of String G str (Lookup G nonterminal))
+          : @of_parse_nonterminal_T str0 str valid nonterminal p h.
           Proof.
             destruct h as [|h]; [ clear; repeat intro; exfalso; omega | ].
             intros pf Hstr Hinit' H_forall.
             let H := match goal with H : str ≤s str0 |- _ => constr:H end in
             destruct (strle_to_sumbool _ H) as [pf_lt|pf_eq].
-            { (** [str] got smaller, so we reset the valid names list *)
-              destruct (@minimal_parse_of_productions__of__parse_of_productions str h minimal_parse_of_name__of__parse_of_name str (reflexivity _) initial_names_data (Lookup G name) p (Lt.lt_S_n _ _ pf) (reflexivity _) (snd H_forall)) as [p'|p'].
+            { (** [str] got smaller, so we reset the valid nonterminals list *)
+              destruct (@minimal_parse_of_productions__of__parse_of_productions str h minimal_parse_of_nonterminal__of__parse_of_nonterminal str (reflexivity _) initial_nonterminals_data (Lookup G nonterminal) p (Lt.lt_S_n _ _ pf) (reflexivity _) (snd H_forall)) as [p'|p'].
               { left.
                 exists (MinParseNonTerminalStrLt _ valid _ pf_lt (fst H_forall) (projT1 p'));
                   simpl.
@@ -748,22 +728,22 @@ Section cfg.
                 solve [ apply Lt.lt_n_Sn
                       | assumption
                       | reflexivity ]. } }
-            { (** [str] didn't get smaller, so we cache the fact that we've hit this name already *)
-              destruct (Sumbool.sumbool_of_bool (is_valid_name valid name)) as [ Hvalid | Hinvalid ].
-              { destruct (@minimal_parse_of_productions__of__parse_of_productions str h minimal_parse_of_name__of__parse_of_name str (reflexivity _) (remove_name valid name) (Lookup G name) p (Lt.lt_S_n _ _ pf) (transitivity (R := sub_names_listT is_valid_name) (@sub_names_listT_remove _ is_valid_name _ remove_name_1 _ _) Hinit') (snd H_forall)) as [p'|p'].
+            { (** [str] didn't get smaller, so we cache the fact that we've hit this nonterminal already *)
+              destruct (Sumbool.sumbool_of_bool (is_valid_nonterminal valid nonterminal)) as [ Hvalid | Hinvalid ].
+              { destruct (@minimal_parse_of_productions__of__parse_of_productions str h minimal_parse_of_nonterminal__of__parse_of_nonterminal str (reflexivity _) (remove_nonterminal valid nonterminal) (Lookup G nonterminal) p (Lt.lt_S_n _ _ pf) (transitivity (R := sub_nonterminals_listT) (@sub_nonterminals_listT_remove _ _ _ _) Hinit') (snd H_forall)) as [p'|p'].
                 { left.
                   subst str.
-                  eexists (@MinimalParse.MinParseNonTerminalStrEq _ _ _ _ _ _ _ _ _ _ (fst H_forall) Hvalid (projT1 p')).
+                  eexists (@MinimalParse.MinParseNonTerminalStrEq _ _ _ _ _ _ _ (fst H_forall) Hvalid (projT1 p')).
                   simpl in *.
                   split;
                     [ exact (Le.le_n_S _ _ (fst (projT2 p')))
                     | split;
                       [ exact (fst H_forall)
                       | exact (snd (projT2 p')) ] ]. }
-                { destruct p' as [name' p'].
-                  destruct (string_dec name name') as [|n].
-                  { subst name; simpl in *.
-                    edestruct (@minimal_parse_of_name__of__parse_of_name (S (size_of_parse p)) pf str0 _ valid name' (projT1 (snd p'))) as [p''|p''];
+                { destruct p' as [nonterminal' p'].
+                  destruct (string_dec nonterminal nonterminal') as [|n].
+                  { subst nonterminal; simpl in *.
+                    edestruct (@minimal_parse_of_nonterminal__of__parse_of_nonterminal (S (size_of_parse p)) pf str0 _ valid nonterminal' (projT1 (snd p'))) as [p''|p''];
                     try solve [ apply Lt.lt_n_S, (fst (projT2 (snd p')))
                               | subst; reflexivity
                               | assumption
@@ -789,17 +769,17 @@ Section cfg.
                           | exact (Lt.lt_n_S _ _ (fst (projT2 (snd p')))) ]
                         | exact (snd (projT2 (snd (projT2 p'')))) ]. } }
                   { right.
-                    exists name'.
+                    exists nonterminal'.
                     destruct p' as [p'H p'p].
                     split.
-                    { rewrite remove_name_5 in p'H by assumption.
+                    { rewrite remove_nonterminal_5 in p'H by assumption.
                       exact p'H. }
                     { exists (projT1 p'p).
                       split; [ exact (Lt.lt_S _ _ (fst (projT2 p'p)))
                              | exact (snd (projT2 p'p)) ]. } } } }
-              { (** oops, we already saw this name in the past.  ABORT! *)
+              { (** oops, we already saw this nonterminal in the past.  ABORT! *)
                 right.
-                exists name.
+                exists nonterminal.
                 destruct H_forall.
                 split; [ split; assumption
                        | ].
@@ -810,19 +790,19 @@ Section cfg.
         End step.
 
         Section wf.
-          Definition minimal_parse_of_name__of__parse_of_name
+          Definition minimal_parse_of_nonterminal__of__parse_of_nonterminal
           : forall h
-                   {str0 str valid name}
-                   (p : parse_of String G str (Lookup G name)),
-              @of_parse_name_T str0 str valid name p h
+                   {str0 str valid nonterminal}
+                   (p : parse_of String G str (Lookup G nonterminal)),
+              @of_parse_nonterminal_T str0 str valid nonterminal p h
             := @Fix
                  _ lt lt_wf
-                 (fun h => forall {str0 str valid name}
-                                  (p : parse_of String G str (Lookup G name)),
-                             @of_parse_name_T str0 str valid name p h)
-                 (@minimal_parse_of_name__of__parse_of_name_step).
+                 (fun h => forall {str0 str valid nonterminal}
+                                  (p : parse_of String G str (Lookup G nonterminal)),
+                             @of_parse_nonterminal_T str0 str valid nonterminal p h)
+                 (@minimal_parse_of_nonterminal__of__parse_of_nonterminal_step).
         End wf.
-      End name.
+      End nonterminal.
     End wf_parts.
   End minimize.
 End cfg.
